specs/Hacl.P256.Square.fst
@@ -1,0 +1,131 @@
+module Hacl.P256.Square
+
+open FStar.Mul
+
+open FStar.HyperStack
+open FStar.HyperStack.ST
+
+open Spec.Lib
+open Spec.Lib.IntSeq
+
+open Spec.Lib.IntTypes
+open Spec.Lib.IntBuf
+
+open Spec.Lib.IntSeq.Lemmas
+open Spec.Lib.IntBuf.Lemmas
+
+open P256.S
+open Hacl.P256.Zeros
+open Hacl.P256.Shrink
+
+open FStar.Math.Lemmas
+
+val smallfelem_expand:
+  out:felem -> input:smallfelem -> Stack unit
+    (requires (fun h -> True))
+    (ensures (fun h0 _ h1 -> True))
+
+let smallfelem_expand out input =
+  let input0 = input.(0) in
+  let input1 = input.(1) in
+  let input2 = input.(2) in
+  let input3 = input.(3) in
+  out.(0) <- to_u128 input0;
+  out.(1) <- to_u128 input1;
+  out.(2) <- to_u128 input2;
+  out.(3) <- to_u128 input3
+
+val smallfelem_square:
+  out:longfelem -> small:smallfelem -> Stack unit
+    (requires (fun h -> True))
+    (ensures (fun h0 _ h1 -> True))
+
+let smallfelem_square out small =
+  let small0 = small.(0) in
+  let small1 = small.(1) in
+  let small2 = small.(2) in
+  let small3 = small.(3) in
+
+  let a = mul_wide small0 small0 in
+  let low = to_u128 (to_u64 a) in
+  let high = a >>. u32(64) in
+  let out0 = low in
+  let out1 = high in
+
+  let a = mul_wide small0 small1 in
+  let low = to_u128 (to_u64 a) in
+  let high = a >>. u32(64) in
+  let out1 = out1 +! low in
+  let out1 = out1 +! low in
+  let out2 = high in
+
+  let a = mul_wide small0 small2 in
+  let low = to_u128 (to_u64 a) in
+  let high = a >>. u32(64) in
+  let out2 = out2 +! low in
+  let out2 = out2 <<. u32(1) in
+  let out3 = high in
+
+  let a = mul_wide small0 small3 in
+  let low = to_u128 (to_u64 a) in
+  let high = a >>. u32(64) in
+  let out3 = out3 +! low in
+  let out4 = high in
+
+  let a = mul_wide small1 small2 in
+  let low = to_u128 (to_u64 a) in
+  let high = a >>. u32(64) in
+  let out3 = out3 +! low in
+  let out3 = out3 <<. u32(1) in
+  let out4 = out4 +! high in
+
+  let a = mul_wide small1 small1 in
+  let low = to_u128 (to_u64 a) in
+  let high = a >>. u32(64) in
+  let out2 = out2 +! low in
+  let out3 = out3 +! high in
+
+  let a = mul_wide small1 small3 in
+  let low = to_u128 (to_u64 a) in
+  let high = a >>. u32(64) in
+  let out4 = out4 +! low in
+  let out4 = out4 <<. u32(1) in
+  let out5 = high in
+
+  let a = mul_wide small2 small3 in
+  let low = to_u128 (to_u64 a) in
+  let high = a >>. u32(64) in
+  let out5 = out5 +! low in
+  let out5 = out5 <<. u32(1) in
+  let out6 = high in
+  let out6 = out6 +! high in
+
+  let a = mul_wide small2 small2 in
+  let low = to_u128 (to_u64 a) in
+  let high = a >>. u32(64) in
+  let out4 = out4 +! low in
+  let out5 = out5 +! high in
+
+  let a = mul_wide small3 small3 in
+  let low = to_u128 (to_u64 a) in
+  let high = a >>. u32(64) in
+  let out6 = out6 +! low in
+  let out7 = high in
+
+  out.(0) <- out0;
+  out.(1) <- out1;
+  out.(2) <- out2;
+  out.(3) <- out3;
+  out.(4) <- out4;
+  out.(5) <- out5;
+  out.(6) <- out6;
+  out.(7) <- out7
+
+val felem_square:
+  out:longfelem -> input:felem ->small: smallfelem -> Stack unit
+    (requires (fun h -> True))
+    (ensures (fun h0 _ h1 -> True))
+
+let felem_square out input small =
+  felem_shrink small input;
+  smallfelem_square out small
